Implement `semiOutParamPos` and `semiOutParamNeg`

Iris/Iris/Algebra/IsOp.lean
@@ -23,17 +23,16 @@ section IsOp
 -/
 @[ipm_class, rocq_alias IsOp, rocq_alias IsOp', rocq_alias IsOp'LR]
 class IsOp [CMRA α]
-    (_ : InOut) (a : semiOutParam α)
-    (_ : InOut) (b1 : semiOutParam α)
-    (_ : InOut) (b2 : semiOutParam α) where
+    (io : InOut) (a : semiOutParamPos io α)
+    (b1 : semiOutParamNeg io α)
+    (b2 : semiOutParamNeg io α) where
   is_op : a ≡ b1 • b2
 
 /--
   Syntactic sugar for specifying whether `IsOp` is used for merging or splitting.
 -/
-abbrev IsOpMerge [CMRA α] (a b1 b2 : semiOutParam α) := IsOp .out a .in b1 .in b2
-abbrev IsOpSplit [CMRA α] (a b1 b2 : semiOutParam α) := IsOp .in a .out b1 .out b2
-
+abbrev IsOpMerge [CMRA α] (a b1 b2 : α) := IsOp .out a b1 b2
+abbrev IsOpSplit [CMRA α] (a b1 b2 : α) := IsOp .in a b1 b2
 
 set_option synthInstance.checkSynthOrder false in
 /--
@@ -60,31 +59,31 @@ instance (priority := default + 100) isOpSplit_op [CMRA α] (a b : α) :
 -/
 
 @[rocq_alias is_op_pair]
-instance isOp_pair [CMRA α] {ioa iob1 iob2 : InOut}
+instance isOp_pair [CMRA α] {io : InOut}
     (a b1 b2 : α) (a' b1' b2' : α)
-    [h1 : IsOp ioa a iob1 b1 iob2 b2] [h2 : IsOp ioa a' iob1 b1' iob2 b2'] :
-    IsOp ioa (a, a') iob1 (b1, b1') iob2 (b2, b2') where
+    [h1 : IsOp io a b1 b2] [h2 : IsOp io a' b1' b2'] :
+    IsOp io (a, a') (b1, b1') (b2, b2') where
   is_op := OFE.equiv_prod_ext h1.is_op h2.is_op
 
 set_option synthInstance.checkSynthOrder false in
 @[rocq_alias is_op_pair_core_id_l]
-instance isOp_pair_core_id_l [CMRA α] [CMRA β] {ioa iob1 iob2 : InOut}
-    (a : α) (a' b1' b2' : β) [h1 : CoreId a] [h2 : IsOp ioa a' iob1 b1' iob2 b2'] :
-    IsOp ioa (a, a') iob1 (a, b1') iob2 (a, b2') where
+instance isOp_pair_core_id_l [CMRA α] [CMRA β] {io : InOut}
+    (a : α) (a' b1' b2' : β) [h1 : CoreId a] [h2 : IsOp io a' b1' b2'] :
+    IsOp io (a, a') (a, b1') (a, b2') where
   is_op := OFE.equiv_prod_ext (op_self a).symm h2.is_op
 
 set_option synthInstance.checkSynthOrder false in
 @[rocq_alias is_op_pair_core_id_r]
-instance isOpMerge_pair_core_id_r [CMRA α] [CMRA β] {ioa iob1 iob2 : InOut}
+instance isOpMerge_pair_core_id_r [CMRA α] [CMRA β] {io : InOut}
     (a b1 b2 : α) (a' : β)
-    [h1 : CoreId a'] [h2 : IsOp ioa a iob1 b1 iob2 b2] :
-    IsOp ioa (a, a') iob1 (b1, a') iob2 (b2, a') where
+    [h1 : CoreId a'] [h2 : IsOp io a b1 b2] :
+    IsOp io (a, a') (b1, a') (b2, a') where
   is_op := OFE.equiv_prod_ext h2.is_op (op_self a').symm
 
 @[rocq_alias is_op_Some]
-instance isOp_some [CMRA α] (a b1 b2 : α) {ioa iob1 iob2 : InOut}
-    [h : IsOp ioa a iob1 b1 iob2 b2] :
-    IsOp ioa (some a) iob1 (some b1) iob2 (some b2) where
+instance isOp_some [CMRA α] (a b1 b2 : α) {io : InOut}
+    [h : IsOp io a b1 b2] :
+    IsOp io (some a) (some b1) (some b2) where
   is_op := h.is_op
 
 end IsOp
