Iris/Iris/ProofMode/Classes.lean
@@ -27,16 +27,19 @@ inductive AsEmpValid.Direction where
   | from
 
 @[ipm_class, rocq_alias AsEmpValid]
-class AsEmpValid (d : AsEmpValid.Direction) (φ : Prop) (_ : InOut) (PROP : semiOutParam $ Type _)
-(_ : InOut) (bi : semiOutParam $ BI PROP) (P : outParam $ PROP) where
+class AsEmpValid (d : AsEmpValid.Direction) (φ : Prop) (io : InOut)
+    (PROP : semiOutParamPos io $ Type _)
+    (bi : semiOutParamPos io $ BI PROP) (P : outParam $ PROP) where
   as_emp_valid : (d = .into → φ → ⊢ P) ∧ (d = .from → (⊢ P) → φ)
 
 @[rocq_alias as_emp_valid_1]
-theorem asEmpValid_1 {PROP} [bi : BI PROP] {φ : Prop} (P : PROP) [AsEmpValid .into φ .in PROP .in bi P]
-: φ → ⊢ P := (AsEmpValid.as_emp_valid .in .in).1 rfl
+theorem asEmpValid_1 {PROP} [bi : BI PROP] {φ : Prop} (P : PROP)
+    [inst : AsEmpValid .into φ .in PROP bi P] : φ → ⊢ P :=
+  inst.as_emp_valid.left rfl
 @[rocq_alias as_emp_valid_2]
-theorem asEmpValid_2 {PROP} [bi : BI PROP] {P: PROP} (φ : Prop) [AsEmpValid .from φ .out PROP .out bi P]
-: (⊢ P) → φ := (AsEmpValid.as_emp_valid .out .out).2 rfl
+theorem asEmpValid_2 {PROP} [bi : BI PROP] {P: PROP} (φ : Prop)
+    [inst : AsEmpValid .from φ .out PROP bi P] : (⊢ P) → φ :=
+  inst.as_emp_valid.right rfl
 
 /- Depending on the use case, type classes with the prefix `From` or `Into` are used. Type classes
 with the prefix `From` are used to generate one or more propositions *from* which the original
@@ -50,7 +53,8 @@ class FromImp {PROP} [BI PROP] (P : PROP) (Q1 Q2 : outParam $ PROP) where
 export FromImp (from_imp)
 
 @[ipm_class, rocq_alias FromWand]
-class FromWand {PROP} [BI PROP] (P : PROP) (_ : InOut) (Q1 : semiOutParam PROP) (Q2 : outParam $ PROP) where
+class FromWand {PROP} [BI PROP] (P : PROP) (io : InOut)
+    (Q1 : semiOutParamPos io PROP) (Q2 : outParam $ PROP) where
   from_wand : (Q1 -∗ Q2) ⊢ P
 export FromWand (from_wand)
 
@@ -58,8 +62,8 @@ export FromWand (from_wand)
 
 @[ipm_class, rocq_alias IntoWand]
 class IntoWand {PROP} [BI PROP] (p q : Bool) (R : PROP)
-  (ioP : InOut) (P : semiOutParam PROP)
-  (ioQ : InOut) (Q : semiOutParam PROP) where
+  (ioP : InOut) (P : semiOutParamPos ioP PROP)
+  (ioQ : InOut) (Q : semiOutParamPos ioQ PROP) where
   into_wand : □?p R ⊢ □?q P -∗ Q
 export IntoWand (into_wand)
 
@@ -134,7 +138,8 @@ class IntoAbsorbingly {PROP} [BI PROP] (P : outParam $ PROP) (Q : PROP) where
 export IntoAbsorbingly (into_absorbingly)
 
 @[ipm_class, rocq_alias FromAssumption, rocq_alias KnownLFromAssumption, rocq_alias KnownRFromAssumption]
-class FromAssumption {PROP} [BI PROP] (p : Bool) (ioP : InOut) (P : semiOutParam $ PROP) (Q : PROP) where
+class FromAssumption {PROP} [BI PROP] (p : Bool) (ioP : InOut)
+    (P : semiOutParamPos ioP PROP) (Q : PROP) where
   from_assumption : □?p P ⊢ Q
 export FromAssumption (from_assumption)
 
@@ -146,7 +151,8 @@ export IntoPure (into_pure)
 #rocq_ignore into_pureT_hint "IntoPureT is not necessary in Lean"
 
 @[ipm_class, rocq_alias FromPure, rocq_alias FromPureT]
-class FromPure {PROP} [BI PROP] (a : outParam $ Bool) (P : PROP) (ioφ : InOut) (φ : semiOutParam $ Prop) where
+class FromPure {PROP} [BI PROP] (a : outParam $ Bool) (P : PROP) (ioφ : InOut)
+    (φ : semiOutParamPos ioφ Prop) where
   from_pure : <affine>?a ⌜φ⌝ ⊢ P
 export FromPure (from_pure)
 
