Iris/Iris/Algebra/Auth.lean
@@ -137,10 +137,9 @@ nonrec theorem auth_dfrac_op {dq1 dq2 : DFrac} {a : A} :
     (●{dq1 • dq2} a) ≡ (●{dq1} a) • (●{dq2} a) :=
   auth_op_auth_eqv
 
-set_option synthInstance.checkSynthOrder false in
 @[rocq_alias auth_auth_dfrac_is_op]
-instance {dq dq1 dq2 : DFrac} [h : IsOp io1 dq io2 dq1 io3 dq2] :
-    IsOp io1 (●{dq} a : Auth A) io2 (●{dq1} a) io3 (●{dq2} a) where
+instance {dq dq1 dq2 : DFrac} {a : A} [h : IsOp io dq dq1 dq2] :
+    IsOp io (●{dq} a : Auth A) (●{dq1} a) (●{dq2} a) where
   is_op := by
     rw [h.is_op.to_eq]
     apply auth_dfrac_op
@@ -181,8 +180,8 @@ nonrec instance {a : A} {b : A} [CoreId b] :
   instCoreIdOpAuthDiscardFrag
 
 @[rocq_alias auth_frag_is_op]
-instance {a b1 b2 : A} [h : IsOp io1 a io2 b1 io3 b2] :
-    IsOp io1 (◯ a : Auth A) io2 (◯ b1) io3 (◯ b2) where
+instance {a b1 b2 : A} [h : IsOp io a b1 b2] :
+    IsOp io (◯ a : Auth A) (◯ b1) (◯ b2) where
   is_op := NonExpansive₂.eqv .rfl h.is_op
 
 -- TODO: auth_frag_sep_homomorphism
