Iris/Iris/Algebra/Frac.lean
@@ -153,13 +153,11 @@ theorem Frac.op_eq (p q : Qp) : p • q = p + q := rfl
 @[rocq_alias frac_valid]
 theorem Frac.valid_iff {p : Qp} : ✓ p ↔ p.val ≤ 1 := .rfl
 
-set_option synthInstance.checkSynthOrder false in
 @[rocq_alias frac_is_op]
 instance (priority := default - 10) (q1 q2 : Qp) :
     IsOpMerge (q1 + q2 : Qp) q1 q2 where
   is_op := .rfl
 
-set_option synthInstance.checkSynthOrder false in
 @[rocq_alias is_op_frac]
-instance (q : Qp) : IsOp io1 q io2 q.half io3 q.half where
+instance (q : Qp) : IsOp io q q.half q.half where
   is_op := by refine OFE.Equiv.of_eq (q.ext ?_); grind
